src/n-bit/wordsLib.sml
@@ -182,6 +182,7 @@ val word_asr_compute =
 
 val thms =
   [numeralTheory.numeral_funpow, pairTheory.UNCURRY_DEF,
+   SUC_RULE rich_listTheory.GENLIST, rich_listTheory.SNOC, combinTheory.K_THM,
    iBITWISE, NUMERAL_BITWISE, LSB_def, BITV_def, SBIT_def,
    NUM_RULE [BIT_ZERO] `n` SIGN_EXTEND_def,
    DIVMOD_2EXP, NUMERAL_DIV_2EXP, NUMERAL_TIMES_2EXP, NUMERAL_iDIV2,
@@ -193,11 +194,12 @@ val thms =
    NUM_RULE [NUMERAL_DIV_2EXP,numeralTheory.MOD_2EXP] `n` SLICE_def,
    (SIMP_RULE std_ss [GSYM ODD_MOD2_LEM,arithmeticTheory.MOD_2EXP_def,
       BITS_def,SUC_SUB] o NUM_RULE [BITS_ZERO2] `n`) BIT_def,
-   INT_MIN_SUM, SUC_RULE MOD_2EXP_EQ,
+   INT_MIN_SUM, SUC_RULE MOD_2EXP_EQ, SUC_RULE BOOLIFY_def,
    numeral_log2,numeral_ilog2,LOG_compute,LOWEST_SET_BIT_compute,
    n2w_w2n, w2n_n2w_compute, MOD_WL1 w2w_n2w, Q.SPEC `^n2w ^n` sw2sw_def,
    word_len_def, word_L_def, word_H_def, word_T_def,
    word_join_def, SPECL [`^n2w ^n`,`n2w ^m:'b word`] word_concat_def,
+   SPEC `^a` word_replicate_concat_word_list, concat_word_list_def,
    word_reverse_n2w, word_modify_n2w, SPEC `^a` word_log2_n2w,
    word_1comp_n2w, word_or_n2w, word_xor_n2w, word_and_n2w,
    word_2comp_compute, word_sub_def, word_div_def, word_sdiv_def, word_mod_def,
@@ -208,6 +210,8 @@ val thms =
    word_lsb_n2w, word_msb_n2w, word_bit_n2w, fcp_n2w,
    NUM_RULE [DIMINDEX_GT_0] `i` word_index_n2w,
    word_bits_n2w, word_signed_bits_n2w, word_slice_n2w, word_extract_n2w,
+   word_reduce_n2w, Q.SPEC `^n2w ^n` reduce_and, Q.SPEC `^n2w ^n` reduce_or,
+   reduce_xor_def, reduce_xnor_def, reduce_nand_def, reduce_nor_def,
    word_ge_n2w, word_gt_n2w, word_hi_n2w, word_hs_n2w,
    word_le_n2w, word_lo_n2w, word_ls_n2w, word_lt_n2w,
    l2n_def,n2l_def,s2n_def,n2s_def,l2w_def,w2l_def,s2w_def,w2s_def,
@@ -275,13 +279,16 @@ local
   end
 
   val l1 =
-     ["l2w","w2l","s2w","w2s",
+     ["l2w","w2l","s2w","w2s","add_with_carry",
       "word_from_bin_list","word_from_oct_list","word_from_dec_list",
       "word_from_hex_list","word_to_bin_list","word_to_oct_list",
       "word_to_dec_list","word_to_hex_list","word_from_bin_string",
       "word_from_oct_string","word_from_dec_string","word_from_hex_string",
       "word_to_bin_string","word_to_oct_string","word_to_dec_string",
       "word_to_hex_string",
+      "word_reduce", "reduce_and", "reduce_or", "reduce_xor",
+      "reduce_nand", "reduce_nor", "reduce_xnor",
+      "word_replicate", "concat_word_list",
       "w2w","w2n","sw2sw","word_log2","word_reverse","word_msb",
       "word_join","word_concat","word_bit","word_bits","word_signed_bits",
       "word_slice","word_extract","word_asr","word_lsr","word_lsl","word_ror",
@@ -290,7 +297,7 @@ local
   val l2 =
      ["l2n","n2l","s2n","n2s","HEX","UNHEX","SBIT","BIT","BITS","BITV",
       "SLICE","TIMES_2EXP","DIVMOD_2EXP","LSB","LOG2","LOG","BITWISE",
-      "BIT_REVERSE","SIGN_EXTEND",
+      "BIT_REVERSE","SIGN_EXTEND", "BOOLIFY",
       "num_from_bin_list","num_from_oct_list","num_from_dec_list",
       "num_from_hex_list","num_to_bin_list","num_to_oct_list",
       "num_to_dec_list","num_to_hex_list","num_from_bin_string",
@@ -298,20 +305,25 @@ local
       "num_to_bin_string","num_to_oct_string","num_to_dec_string",
       "num_to_hex_string"]
 
-  val s = name_thy_set (("min","=")::("arithmetic","DIV_2EXP") ::
+  val s = name_thy_set
+           (("min","=")::("arithmetic","DIV_2EXP") ::("fcp","fcp_index")::
              map (pair "words") l1 @ map (pair "bit") l2)
 
   fun is_hex_digit_literal t =
         numSyntax.is_numeral t andalso
         numSyntax.int_of_term t < 16;
 
-  fun is_hex_digit_list t =
-        listSyntax.is_list t andalso
-        all is_hex_digit_literal (fst (listSyntax.dest_list t));
-
-  fun is_hex_string t =
-        stringSyntax.is_string_literal t andalso
-        all Char.isHexDigit (String.explode (stringSyntax.fromHOLstring t));
+  fun is_ground_list t =
+         let val (l,ty) = listSyntax.dest_list t in
+           if ty = ``:num`` then
+             Lib.all is_hex_digit_literal l
+           else if ty = ``:char`` then
+             Lib.all (Char.isHexDigit o stringSyntax.fromHOLchar) l
+           else if ty = ``:bool`` then
+             Lib.all (fn tm => term_eq F tm orelse term_eq T tm) l
+           else
+             wordsSyntax.is_word_type ty
+         end handle HOL_ERR _ => false;
 
   fun is_ground_arg t =
     if pairSyntax.is_pair t then
@@ -322,10 +334,9 @@ local
       numSyntax.is_numeral t orelse
       wordsSyntax.is_word_literal t orelse
       is_uintmax t orelse
-      is_hex_digit_list t orelse
-      is_hex_string t orelse
       term_eq t T orelse
       term_eq t F orelse
+      is_ground_list t orelse
       term_eq t ``bit$HEX`` orelse
       term_eq t ``bit$UNHEX`` orelse
       term_eq t ``bool$/\`` orelse
@@ -338,7 +349,7 @@ local
           val typ = type_of (prim_mk_const{Name=name,Thy=thy})
       in
          (length (fst (strip_fun typ)) = length l) andalso
-         Redblackset.member(s,tn) andalso all is_ground_arg l
+         Redblackset.member(s,tn) andalso Lib.all is_ground_arg l
       end
 
   val alpha_rws =
@@ -985,7 +996,12 @@ val WORD_MUL_LSL_ss =
 val LET_RULE = SIMP_RULE (bool_ss++boolSimps.LET_ss) [];
 val OR_AND_COMM_RULE = ONCE_REWRITE_RULE [WORD_ADD_COMM, WORD_OR_COMM];
 
-val WORD_EXTRACT_ss =
+val WORD_REPLICATE_ss =
+  simpLib.conv_ss
+    {conv = K (K (WORD_EVAL_CONV)), trace = 3, name = "WORD_EVAL_CONV",
+     key = SOME([], ``words$word_replicate ^a ^w:'a word``)};
+
+val WORD_EXTRACT_ss = simpLib.merge_ss [WORD_REPLICATE_ss,
   rewrites ([WORD_EXTRACT_ZERO, WORD_EXTRACT_ZERO2, WORD_EXTRACT_ZERO3,
       WORD_EXTRACT_LSL, word_concat_def, LET_RULE word_join_def,
       word_rol_def, LET_RULE word_ror, word_asr, word_lsr_n2w,
@@ -998,7 +1014,7 @@ val WORD_EXTRACT_ss =
       (GEN_ALL o ISPEC `words$word_extract h l :'a word -> 'b word`) COND_RAND,
       WORD_BITS_EXTRACT, WORD_w2w_EXTRACT, sw2sw_w2w, word_lsb, word_msb] @
     map (REWRITE_RULE [WORD_BITS_EXTRACT])
-     [WORD_ALL_BITS, WORD_SLICE_THM, WORD_BIT_BITS]);
+     [WORD_ALL_BITS, WORD_SLICE_THM, WORD_BIT_BITS])];
 
 (* ------------------------------------------------------------------------- *)
 
@@ -1074,7 +1090,7 @@ local
              SPEC `^a` n2w_def, pred_setTheory.NOT_IN_EMPTY,
              ISPEC `0n` pred_setTheory.IN_INSERT,
              ISPEC `^a` pred_setTheory.IN_INSERT]
-  val rw2 = [fcpTheory.FCP_UPDATE_def,LESS_COR,sw2sw,w2w,
+  val rw2 = [fcpTheory.FCP_UPDATE_def,LESS_COR,sw2sw,w2w,word_replicate_def,
              word_join,word_concat_def,word_reverse_def,word_modify_def,
              word_lsl_def,word_lsr_def,word_asr_def,word_ror_def,
              word_rol_def,word_rrx_def,word_msb_def,word_lsb_def,
@@ -1360,101 +1376,9 @@ fun remove_word_cast_printer () =
   (Parse.remove_user_printer "wordsLib.print_word_cast"; ());
 
 (* ------------------------------------------------------------------------- *)
-(* Guessing the word length for the result of extraction (><) and            *)
-(* concatenate (@@)                                                          *)
+(* Guessing the word length for the result of extraction (><),               *)
+(* concatenate (@@), word_replicate and concat_word_list                     *)
 (* ------------------------------------------------------------------------- *)
-
-val extract_tm = ``words$word_extract ^m ^n :'a word -> 'b word``;
-
-datatype WordOp =
-   word_concat of hol_type * hol_type * hol_type
- | word_extract of num * hol_type;
-
-fun get_word_ops t =
-  case total (match_term extract_tm) t of
-    NONE =>
-      (case dest_term t of
-         VAR (a, b) => []
-       | CONST a =>
-           if #Name a = "word_concat" then
-            (case dest_type (#Ty a) of
-               ("fun", [x,y]) =>
-                 (case dest_type y of
-                    ("fun", [v,w]) =>
-                       (let val fv = trye hd (type_vars w)
-                            val xn = wordsSyntax.dest_word_type x
-                            val vn = wordsSyntax.dest_word_type v
-                        in
-                          [word_concat (xn, vn, fv)]
-                        end handle HOL_ERR _ => [])
-                  | _ => [])
-             | _ => [])
-           else
-             []
-       | COMB (a,b) => get_word_ops a @ get_word_ops b
-       | LAMB (a,b) => get_word_ops b)
-  | SOME ([a,b],_) =>
-      (case dest_type (type_of t) of
-         ("fun", [x, y]) =>
-            (let val fv = trye hd (type_vars y)
-                 val na = numSyntax.dest_numeral (#residue a)
-                 val nb = numSyntax.dest_numeral (#residue b)
-                 val n = Arbnum.-(Arbnum.plus1 na, nb)
-             in
-               if n = Arbnum.zero then [] else [word_extract (n, fv)]
-             end handle HOL_ERR _ => [])
-      | _ => [])
-  | _ => [];
-
-fun word_op_compare(a, b) =
-  case (a, b) of
-    (word_concat(a,b,c),word_concat(d,e,f)) =>
-      (case (is_vartype a, is_vartype b, is_vartype d, is_vartype e)
-       of (false,false,true,_) => LESS
-        | (false,false,_,true) => LESS
-        | (true,_,false,false) => GREATER
-        | (_,true,false,false) => GREATER
-        | _ =>
-           (if a = f orelse b = f then
-              if d = c orelse e = c then Type.compare(c, f) else GREATER
-            else
-              if d = c orelse e = c then LESS else Type.compare(c, f)))
-  | (word_concat(a,b,c),word_extract(n,f)) => GREATER
-  | (word_extract(m,c),word_concat(d,e,f)) => LESS
-  | (word_extract(m,c),word_extract(n,f))  => Type.compare(c, f);
-
-local
-  open Redblackmap
-
-  fun mk_word_op_var_map vmap [] = vmap
-    | mk_word_op_var_map vmap (word_extract (n, ty)::tl) =
-       (case peek(vmap, ty) of
-          NONE   => mk_word_op_var_map (insert(vmap,ty,n)) tl
-        | SOME m => mk_word_op_var_map (if Arbnum.<(n, m) then vmap
-                                        else insert(vmap,ty,n)) tl)
-    | mk_word_op_var_map vmap (word_concat (a, b, ty)::tl) =
-       (let val na = if Type.is_vartype a then
-                       trye find (vmap, a)
-                     else
-                       fcpLib.index_to_num a
-            val nb = if Type.is_vartype b then
-                       trye find (vmap, b)
-                     else
-                       fcpLib.index_to_num b
-            val n = Arbnum.+(na, nb)
-        in
-          case peek(vmap, ty) of
-            NONE   => mk_word_op_var_map (insert(vmap,ty,n)) tl
-          | SOME m => mk_word_op_var_map (if Arbnum.<(n, m) then vmap
-                                          else insert(vmap,ty,n)) tl
-        end handle HOL_ERR _ => mk_word_op_var_map vmap tl)
-in
-  fun mk_vmap t = mk_word_op_var_map (mkDict Type.compare)
-                    (Listsort.sort word_op_compare (get_word_ops t))
-end;
-
-fun word_op_type_inst (ty:hol_type, n) =
-  {redex = ty, residue = fcpLib.index_type n};
 
 val notify_on_word_length_guess = ref true;
 val guessing_word_lengths = ref false;
@@ -1465,34 +1389,68 @@ val _ = Feedback.register_btrace("notify word length guesses",
 val _ = Feedback.register_btrace("guess word lengths",
                                   guessing_word_lengths);
 
-local
-  fun comma_separate_acc [] l = l
-    | comma_separate_acc (h::t) "" = comma_separate_acc t h
-    | comma_separate_acc [h] l = l ^ " and " ^ h
-    | comma_separate_acc (h::t) l = comma_separate_acc t (l ^ ", " ^ h)
-  fun comma_separate l = comma_separate_acc l ""
+fun guess_lengths ()      = set_trace "guess word lengths" 1;
+fun dont_guess_lengths () = set_trace "guess word lengths" 0;
 
-  fun type_name t = String.extract(Hol_pp.type_to_string t, 1, NONE);
+fun dest_strip t =
+let val (l,r) = strip_comb t in
+  (fst (dest_const l), r)
+end;
 
-  fun guess_to_string {redex = a, residue = b} =
-    type_name a ^ " <- " ^ type_name b;
+fun t2s t = String.extract(Hol_pp.type_to_string t, 1, NONE);
 
-  fun print_guesses l = Feedback.HOL_MESG
-    ("assigning word length(s): " ^ comma_separate (map guess_to_string l));
+fun LENGTH_INST t =
+let open numSyntax
+    val word_type = wordsSyntax.dest_word_type o type_of
+    val ty = word_type t
 in
-  fun inst_word_lengths t =
-  let val assigns = map word_op_type_inst (Redblackmap.listItems (mk_vmap t))
-      val _ = if !Globals.interactive andalso
-                 !notify_on_word_length_guess andalso
-                 not (null assigns)
-              then
-                print_guesses assigns
-              else
-                ()
-  in
-    inst assigns t
-  end
-end
+  if Type.polymorphic ty then
+    case dest_strip t
+    of ("word_extract", [h,l,_]) =>
+          let val nh = dest_numeral h
+              val nl = dest_numeral l
+              val nt = Arbnum.- (Arbnum.plus1 nh, nl)
+          in
+            ty |-> fcpLib.index_type nt
+          end
+     | ("word_concat", [a,b]) =>
+          let val na = fcpLib.index_to_num (word_type a)
+              val nb = fcpLib.index_to_num (word_type b)
+              val nt = Arbnum.+ (na, nb)
+          in
+            ty |-> fcpLib.index_type nt
+          end
+     | ("word_replicate", [m,a]) =>
+          let val nm = dest_numeral m
+              val na = fcpLib.index_to_num (word_type a)
+              val nt = Arbnum.* (nm, na)
+          in
+            ty |-> fcpLib.index_type nt
+          end
+     | ("concat_word_list", [l]) =>
+          let val (ls,tyl) = listSyntax.dest_list l
+              val nl = fcpLib.index_to_num (wordsSyntax.dest_word_type tyl)
+              val nt = Arbnum.* (Arbnum.fromInt (length ls), nl)
+          in
+            ty |-> fcpLib.index_type nt
+          end
+     | _ => raise ERR "LENGTH_INST" ""
+  else
+    raise ERR "LENGTH_INST" ""
+end;
+
+fun inst_word_lengths tm =
+let val t = HolKernel.find_term (Lib.can LENGTH_INST) tm
+    val {redex,residue} = LENGTH_INST t
+    val _ = if !Globals.interactive andalso !notify_on_word_length_guess then
+              Feedback.HOL_MESG
+                (String.concat ["assigning word length: ",
+                                t2s redex, " <- ", t2s residue])
+            else
+              ()
+in
+  inst_word_lengths (Term.inst [redex |-> residue] tm)
+end handle HOL_ERR _ => tm;
 
 fun word_post_process_term t =
   if !guessing_word_lengths then
@@ -1502,9 +1460,6 @@ fun word_post_process_term t =
 
 val _ = Parse.post_process_term :=
   (word_post_process_term o !Parse.post_process_term);
-
-fun guess_lengths ()      = set_trace "guess word lengths" 1;
-fun dont_guess_lengths () = set_trace "guess word lengths" 0;
 
 val operators = [("+", "word_add"), ("-", "word_sub"),
                  ("numeric_negate", "word_2comp"),
