src/pair/src/pairLib.sig
@@ -75,6 +75,7 @@ sig
  val PAIRED_ETA_CONV  : conv
  val GEN_BETA_CONV    : conv
  val let_CONV         : conv
+ val LET_SIMP_CONV    : bool -> conv
  val GEN_BETA_RULE    : thm -> thm
  val GEN_BETA_TAC     : tactic
 
